Empty and nonempty sums

HOL-ETCS/Summation.thy
@@ -638,62 +638,113 @@ proof -
 qed
 
 definition summation :: cfunc where
-  "summation  = (zero \<amalg> (indexed_sum \<circ>\<^sub>c \<langle>\<langle>left_cart_proj \<nat>\<^sub>c \<nat>\<^sub>c \<circ>\<^sub>c (left_cart_proj (\<nat>\<^sub>c \<times>\<^sub>c \<nat>\<^sub>c) (\<nat>\<^sub>c\<^bsup>\<nat>\<^sub>c\<^esup>)),  
+"summation  = ((indexed_sum \<circ>\<^sub>c \<langle>\<langle>left_cart_proj \<nat>\<^sub>c \<nat>\<^sub>c \<circ>\<^sub>c (left_cart_proj (\<nat>\<^sub>c \<times>\<^sub>c \<nat>\<^sub>c) (\<nat>\<^sub>c\<^bsup>\<nat>\<^sub>c\<^esup>)),  
                                 right_cart_proj (\<nat>\<^sub>c \<times>\<^sub>c \<nat>\<^sub>c) (\<nat>\<^sub>c\<^bsup>\<nat>\<^sub>c\<^esup>)\<rangle>, 
-                                monus2 \<circ>\<^sub>c \<langle>(right_cart_proj \<nat>\<^sub>c \<nat>\<^sub>c) \<circ>\<^sub>c (left_cart_proj (\<nat>\<^sub>c \<times>\<^sub>c \<nat>\<^sub>c) (\<nat>\<^sub>c\<^bsup>\<nat>\<^sub>c\<^esup>)), 
-                                           (left_cart_proj \<nat>\<^sub>c \<nat>\<^sub>c) \<circ>\<^sub>c (left_cart_proj (\<nat>\<^sub>c \<times>\<^sub>c \<nat>\<^sub>c) (\<nat>\<^sub>c\<^bsup>\<nat>\<^sub>c\<^esup>))\<rangle>\<rangle>))
-                 \<circ>\<^sub>c (case_bool \<circ>\<^sub>c leq \<circ>\<^sub>c \<langle>left_cart_proj \<nat>\<^sub>c \<nat>\<^sub>c, right_cart_proj \<nat>\<^sub>c \<nat>\<^sub>c\<rangle> \<times>\<^sub>f id (\<nat>\<^sub>c\<^bsup>\<nat>\<^sub>c\<^esup>))"
-
-lemma something_easier:
-  "case_bool \<circ>\<^sub>c leq \<circ>\<^sub>c \<langle>left_cart_proj \<nat>\<^sub>c \<nat>\<^sub>c, right_cart_proj \<nat>\<^sub>c \<nat>\<^sub>c\<rangle> : \<nat>\<^sub>c \<times>\<^sub>c \<nat>\<^sub>c \<rightarrow> (\<one> \<Coprod> \<one>)"
-  by typecheck_cfuncs
-
-lemma something_easy:
-  "\<langle>id (\<nat>\<^sub>c \<times>\<^sub>c \<nat>\<^sub>c), (case_bool \<circ>\<^sub>c leq \<circ>\<^sub>c \<langle>left_cart_proj \<nat>\<^sub>c \<nat>\<^sub>c, right_cart_proj \<nat>\<^sub>c \<nat>\<^sub>c\<rangle>)\<rangle> \<times>\<^sub>f id (\<nat>\<^sub>c\<^bsup>\<nat>\<^sub>c\<^esup>) :
-                           (\<nat>\<^sub>c \<times>\<^sub>c \<nat>\<^sub>c) \<times>\<^sub>c (\<nat>\<^sub>c\<^bsup>\<nat>\<^sub>c\<^esup>) \<rightarrow> ((\<nat>\<^sub>c \<times>\<^sub>c \<nat>\<^sub>c) \<times>\<^sub>c (\<one> \<Coprod> \<one>)) \<times>\<^sub>c (\<nat>\<^sub>c\<^bsup>\<nat>\<^sub>c\<^esup>)"
-  by typecheck_cfuncs
-
-lemma something_easy_on_elements:
-  assumes l_type[type_rule]: "l \<in>\<^sub>c \<nat>\<^sub>c"
-  assumes u_type[type_rule]: "u \<in>\<^sub>c \<nat>\<^sub>c"
-  assumes "l \<le>\<^sub>\<nat> u"
-  assumes f_type[type_rule]: "f \<in>\<^sub>c \<nat>\<^sub>c\<^bsup>\<nat>\<^sub>c\<^esup>"
-  shows "(\<langle>id (\<nat>\<^sub>c \<times>\<^sub>c \<nat>\<^sub>c), (case_bool \<circ>\<^sub>c leq \<circ>\<^sub>c \<langle>left_cart_proj \<nat>\<^sub>c \<nat>\<^sub>c, right_cart_proj \<nat>\<^sub>c \<nat>\<^sub>c\<rangle>)\<rangle> \<times>\<^sub>f id (\<nat>\<^sub>c\<^bsup>\<nat>\<^sub>c\<^esup>)) \<circ>\<^sub>c \<langle>\<langle>l,u\<rangle>,f\<rangle>=
-          \<langle>\<langle>\<langle>l,u\<rangle>, left_coproj \<one> \<one>\<rangle>, f\<rangle>"
-  using assms apply typecheck_cfuncs
-  by (smt (verit, ccfv_SIG) assms(3) case_bool_true cfunc_cross_prod_comp_cfunc_prod cfunc_prod_comp cfunc_prod_unique comp_associative2 id_left_unit2 id_right_unit2 leq_infix_def)
-        
+                                monus2 \<circ>\<^sub>c swap \<nat>\<^sub>c \<nat>\<^sub>c \<circ>\<^sub>c left_cart_proj (\<nat>\<^sub>c \<times>\<^sub>c \<nat>\<^sub>c) (\<nat>\<^sub>c\<^bsup>\<nat>\<^sub>c\<^esup>)
+\<rangle>)
+              \<amalg>
+              (zero \<circ>\<^sub>c \<beta>\<^bsub>(\<nat>\<^sub>c \<times>\<^sub>c \<nat>\<^sub>c) \<times>\<^sub>c (\<nat>\<^sub>c\<^bsup>\<nat>\<^sub>c\<^esup>)\<^esub>)) \<circ>\<^sub>c cases  (leq \<circ>\<^sub>c left_cart_proj (\<nat>\<^sub>c \<times>\<^sub>c \<nat>\<^sub>c) (\<nat>\<^sub>c\<^bsup>\<nat>\<^sub>c\<^esup>))"
 
 
+lemma type_1[type_rule]: 
+  "cases  (leq \<circ>\<^sub>c left_cart_proj (\<nat>\<^sub>c \<times>\<^sub>c \<nat>\<^sub>c) (\<nat>\<^sub>c\<^bsup>\<nat>\<^sub>c\<^esup>)) : (\<nat>\<^sub>c \<times>\<^sub>c \<nat>\<^sub>c) \<times>\<^sub>c (\<nat>\<^sub>c\<^bsup>\<nat>\<^sub>c\<^esup>) \<rightarrow> ((\<nat>\<^sub>c \<times>\<^sub>c \<nat>\<^sub>c) \<times>\<^sub>c (\<nat>\<^sub>c\<^bsup>\<nat>\<^sub>c\<^esup>)) \<Coprod> ((\<nat>\<^sub>c \<times>\<^sub>c \<nat>\<^sub>c) \<times>\<^sub>c (\<nat>\<^sub>c\<^bsup>\<nat>\<^sub>c\<^esup>))"
+  unfolding cases_def
+  by (metis cases_def cases_type comp_type left_cart_proj_type leq_type) 
 
-(*
 lemma summation_type[type_rule]: 
-  "summation : (\<nat>\<^sub>c \<times>\<^sub>c \<nat>\<^sub>c) \<times>\<^sub>c (\<nat>\<^sub>c\<^bsup>\<nat>\<^sub>c\<^esup>) \<rightarrow> \<nat>\<^sub>c \<times>\<^sub>c (\<nat>\<^sub>c\<^bsup>\<nat>\<^sub>c\<^esup>)"
+  "summation : (\<nat>\<^sub>c \<times>\<^sub>c \<nat>\<^sub>c) \<times>\<^sub>c (\<nat>\<^sub>c\<^bsup>\<nat>\<^sub>c\<^esup>) \<rightarrow>\<nat>\<^sub>c"
   unfolding summation_def by typecheck_cfuncs
-*)
-
-
-(*
+               
 lemma empty_sum:
   assumes l_type[type_rule]: "lower \<in>\<^sub>c \<nat>\<^sub>c"
   assumes u_type[type_rule]: "upper \<in>\<^sub>c \<nat>\<^sub>c"
   assumes "successor \<circ>\<^sub>c upper \<le>\<^sub>\<nat> lower"
   assumes f_type[type_rule]: "f \<in>\<^sub>c \<nat>\<^sub>c\<^bsup>\<nat>\<^sub>c\<^esup>"
   shows "summation \<circ>\<^sub>c \<langle>\<langle>lower, upper\<rangle>, f\<rangle> = zero"
-  unfolding summation_def
+  unfolding summation_def 
 proof - 
-  have "(indexed_sum \<circ>\<^sub>c \<langle>\<langle>left_cart_proj \<nat>\<^sub>c \<nat>\<^sub>c \<circ>\<^sub>c left_cart_proj (\<nat>\<^sub>c \<times>\<^sub>c \<nat>\<^sub>c) (\<nat>\<^sub>c\<^bsup>\<nat>\<^sub>c\<^esup>),
-                         right_cart_proj (\<nat>\<^sub>c \<times>\<^sub>c \<nat>\<^sub>c) (\<nat>\<^sub>c\<^bsup>\<nat>\<^sub>c\<^esup>)\<rangle>,
-           monus2 \<circ>\<^sub>c \<langle>right_cart_proj \<nat>\<^sub>c \<nat>\<^sub>c \<circ>\<^sub>c left_cart_proj (\<nat>\<^sub>c \<times>\<^sub>c \<nat>\<^sub>c) (\<nat>\<^sub>c\<^bsup>\<nat>\<^sub>c\<^esup>),
-                       left_cart_proj \<nat>\<^sub>c \<nat>\<^sub>c \<circ>\<^sub>c left_cart_proj (\<nat>\<^sub>c \<times>\<^sub>c \<nat>\<^sub>c) (\<nat>\<^sub>c\<^bsup>\<nat>\<^sub>c\<^esup>)\<rangle>\<rangle>) \<circ>\<^sub>c  \<langle>\<langle>lower,upper\<rangle>,f\<rangle> =
-        indexed_sum \<circ>\<^sub>c \<langle>\<langle>left_cart_proj \<nat>\<^sub>c \<nat>\<^sub>c \<circ>\<^sub>c left_cart_proj (\<nat>\<^sub>c \<times>\<^sub>c \<nat>\<^sub>c) (\<nat>\<^sub>c\<^bsup>\<nat>\<^sub>c\<^esup>) \<circ>\<^sub>c  \<langle>\<langle>lower,upper\<rangle>,f\<rangle>,
-                         right_cart_proj (\<nat>\<^sub>c \<times>\<^sub>c \<nat>\<^sub>c) (\<nat>\<^sub>c\<^bsup>\<nat>\<^sub>c\<^esup>) \<circ>\<^sub>c  \<langle>\<langle>lower,upper\<rangle>,f\<rangle>\<rangle> ,
-           monus2 \<circ>\<^sub>c \<langle>right_cart_proj \<nat>\<^sub>c \<nat>\<^sub>c \<circ>\<^sub>c left_cart_proj (\<nat>\<^sub>c \<times>\<^sub>c \<nat>\<^sub>c) (\<nat>\<^sub>c\<^bsup>\<nat>\<^sub>c\<^esup>) \<circ>\<^sub>c  \<langle>\<langle>lower,upper\<rangle>,f\<rangle>,
-                       left_cart_proj \<nat>\<^sub>c \<nat>\<^sub>c \<circ>\<^sub>c left_cart_proj (\<nat>\<^sub>c \<times>\<^sub>c \<nat>\<^sub>c) (\<nat>\<^sub>c\<^bsup>\<nat>\<^sub>c\<^esup>) \<circ>\<^sub>c  \<langle>\<langle>lower,upper\<rangle>,f\<rangle>\<rangle>\<rangle>"
-    by (typecheck_cfuncs, smt (verit, best) cfunc_prod_comp comp_associative2)
-  also have "... = indexed_sum \<circ>\<^sub>c \<langle>\<langle>lower, f\<rangle>, (upper \<midarrow>\<^sub>\<nat> lower)\<rangle>"
-    by (typecheck_cfuncs, simp add: left_cart_proj_cfunc_prod monus_def right_cart_proj_cfunc_prod)
-*)
+  have False_case: "(leq \<circ>\<^sub>c left_cart_proj (\<nat>\<^sub>c \<times>\<^sub>c \<nat>\<^sub>c) (\<nat>\<^sub>c\<^bsup>\<nat>\<^sub>c\<^esup>)) \<circ>\<^sub>c \<langle>\<langle>lower, upper\<rangle>, f\<rangle> = \<f>"
+    by (etcs_assocr, typecheck_cfuncs, metis assms(3) left_cart_proj_cfunc_prod leq_infix_def nat_strict_total_order true_false_only_truth_values)
+  have "((indexed_sum \<circ>\<^sub>c \<langle>\<langle>left_cart_proj \<nat>\<^sub>c \<nat>\<^sub>c \<circ>\<^sub>c  left_cart_proj (\<nat>\<^sub>c \<times>\<^sub>c \<nat>\<^sub>c) (\<nat>\<^sub>c\<^bsup>\<nat>\<^sub>c\<^esup>),
+          right_cart_proj (\<nat>\<^sub>c \<times>\<^sub>c \<nat>\<^sub>c) (\<nat>\<^sub>c\<^bsup>\<nat>\<^sub>c\<^esup>)\<rangle>,monus2 \<circ>\<^sub>c swap \<nat>\<^sub>c \<nat>\<^sub>c \<circ>\<^sub>c left_cart_proj (\<nat>\<^sub>c \<times>\<^sub>c \<nat>\<^sub>c) (\<nat>\<^sub>c\<^bsup>\<nat>\<^sub>c\<^esup>)\<rangle>) \<amalg>
+     (zero \<circ>\<^sub>c \<beta>\<^bsub>(\<nat>\<^sub>c \<times>\<^sub>c \<nat>\<^sub>c) \<times>\<^sub>c \<nat>\<^sub>c\<^bsup>\<nat>\<^sub>c\<^esup>\<^esub>) \<circ>\<^sub>c cases (leq \<circ>\<^sub>c left_cart_proj (\<nat>\<^sub>c \<times>\<^sub>c \<nat>\<^sub>c) (\<nat>\<^sub>c\<^bsup>\<nat>\<^sub>c\<^esup>))) \<circ>\<^sub>c \<langle>\<langle>lower,upper\<rangle>,f\<rangle> =  
+        ((indexed_sum \<circ>\<^sub>c \<langle>\<langle>left_cart_proj \<nat>\<^sub>c \<nat>\<^sub>c \<circ>\<^sub>c  left_cart_proj (\<nat>\<^sub>c \<times>\<^sub>c \<nat>\<^sub>c) (\<nat>\<^sub>c\<^bsup>\<nat>\<^sub>c\<^esup>),
+      right_cart_proj (\<nat>\<^sub>c \<times>\<^sub>c \<nat>\<^sub>c) (\<nat>\<^sub>c\<^bsup>\<nat>\<^sub>c\<^esup>)\<rangle>,monus2 \<circ>\<^sub>c swap \<nat>\<^sub>c \<nat>\<^sub>c  \<circ>\<^sub>c left_cart_proj (\<nat>\<^sub>c \<times>\<^sub>c \<nat>\<^sub>c) (\<nat>\<^sub>c\<^bsup>\<nat>\<^sub>c\<^esup>)\<rangle>) \<amalg>
+     (zero \<circ>\<^sub>c \<beta>\<^bsub>(\<nat>\<^sub>c \<times>\<^sub>c \<nat>\<^sub>c) \<times>\<^sub>c \<nat>\<^sub>c\<^bsup>\<nat>\<^sub>c\<^esup>\<^esub>)) \<circ>\<^sub>c
+     cases (leq \<circ>\<^sub>c left_cart_proj (\<nat>\<^sub>c \<times>\<^sub>c \<nat>\<^sub>c) (\<nat>\<^sub>c\<^bsup>\<nat>\<^sub>c\<^esup>)) \<circ>\<^sub>c \<langle>\<langle>lower,upper\<rangle>,f\<rangle>"
+    by(etcs_assocr, typecheck_cfuncs)
+  also have "... = (((indexed_sum \<circ>\<^sub>c \<langle>\<langle>left_cart_proj \<nat>\<^sub>c \<nat>\<^sub>c \<circ>\<^sub>c  left_cart_proj (\<nat>\<^sub>c \<times>\<^sub>c \<nat>\<^sub>c) (\<nat>\<^sub>c\<^bsup>\<nat>\<^sub>c\<^esup>),
+      right_cart_proj (\<nat>\<^sub>c \<times>\<^sub>c \<nat>\<^sub>c) (\<nat>\<^sub>c\<^bsup>\<nat>\<^sub>c\<^esup>)\<rangle>,monus2 \<circ>\<^sub>c swap \<nat>\<^sub>c \<nat>\<^sub>c \<circ>\<^sub>c left_cart_proj (\<nat>\<^sub>c \<times>\<^sub>c \<nat>\<^sub>c) (\<nat>\<^sub>c\<^bsup>\<nat>\<^sub>c\<^esup>)\<rangle>) \<amalg>
+     (zero \<circ>\<^sub>c \<beta>\<^bsub>(\<nat>\<^sub>c \<times>\<^sub>c \<nat>\<^sub>c) \<times>\<^sub>c \<nat>\<^sub>c\<^bsup>\<nat>\<^sub>c\<^esup>\<^esub>)) \<circ>\<^sub>c
+     right_coproj ((\<nat>\<^sub>c \<times>\<^sub>c \<nat>\<^sub>c) \<times>\<^sub>c \<nat>\<^sub>c\<^bsup>\<nat>\<^sub>c\<^esup>) ((\<nat>\<^sub>c \<times>\<^sub>c \<nat>\<^sub>c) \<times>\<^sub>c \<nat>\<^sub>c\<^bsup>\<nat>\<^sub>c\<^esup>)) \<circ>\<^sub>c \<langle>\<langle>lower,upper\<rangle>,f\<rangle>"
+    by (etcs_assocr,typecheck_cfuncs, simp add: False_case false_case)
+  also have "... = (zero \<circ>\<^sub>c \<beta>\<^bsub>(\<nat>\<^sub>c \<times>\<^sub>c \<nat>\<^sub>c) \<times>\<^sub>c \<nat>\<^sub>c\<^bsup>\<nat>\<^sub>c\<^esup>\<^esub>) \<circ>\<^sub>c \<langle>\<langle>lower,upper\<rangle>,f\<rangle>"
+    using right_coproj_cfunc_coprod by (typecheck_cfuncs, presburger)
+  also have "... = zero"
+    by (etcs_assocr, typecheck_cfuncs, simp add: id_right_unit2 terminal_func_comp_elem)
+  then show "((indexed_sum \<circ>\<^sub>c \<langle>\<langle>left_cart_proj \<nat>\<^sub>c \<nat>\<^sub>c \<circ>\<^sub>c left_cart_proj (\<nat>\<^sub>c \<times>\<^sub>c \<nat>\<^sub>c) (\<nat>\<^sub>c\<^bsup>\<nat>\<^sub>c\<^esup>),
+            right_cart_proj (\<nat>\<^sub>c \<times>\<^sub>c \<nat>\<^sub>c) (\<nat>\<^sub>c\<^bsup>\<nat>\<^sub>c\<^esup>)\<rangle>,monus2 \<circ>\<^sub>c swap \<nat>\<^sub>c \<nat>\<^sub>c \<circ>\<^sub>c left_cart_proj (\<nat>\<^sub>c \<times>\<^sub>c \<nat>\<^sub>c) (\<nat>\<^sub>c\<^bsup>\<nat>\<^sub>c\<^esup>)\<rangle>) \<amalg>
+  (zero \<circ>\<^sub>c \<beta>\<^bsub>(\<nat>\<^sub>c \<times>\<^sub>c \<nat>\<^sub>c) \<times>\<^sub>c \<nat>\<^sub>c\<^bsup>\<nat>\<^sub>c\<^esup>\<^esub>) \<circ>\<^sub>c cases (leq \<circ>\<^sub>c left_cart_proj (\<nat>\<^sub>c \<times>\<^sub>c \<nat>\<^sub>c) (\<nat>\<^sub>c\<^bsup>\<nat>\<^sub>c\<^esup>))) \<circ>\<^sub>c \<langle>\<langle>lower,upper\<rangle>,f\<rangle> = zero"
+    using calculation by auto
+qed
+               
+lemma nonempty_sum:
+  assumes l_type[type_rule]: "lower \<in>\<^sub>c \<nat>\<^sub>c"
+  assumes u_type[type_rule]: "upper \<in>\<^sub>c \<nat>\<^sub>c"
+  assumes "lower \<le>\<^sub>\<nat> upper"
+  assumes f_type[type_rule]: "f \<in>\<^sub>c \<nat>\<^sub>c\<^bsup>\<nat>\<^sub>c\<^esup>"
+  shows "summation \<circ>\<^sub>c \<langle>\<langle>lower, upper\<rangle>, f\<rangle> = indexed_sum \<circ>\<^sub>c \<langle>\<langle>lower, f\<rangle>, upper \<midarrow>\<^sub>\<nat> lower\<rangle>"
+  unfolding summation_def 
+proof -
+  have True_case: "(leq \<circ>\<^sub>c left_cart_proj (\<nat>\<^sub>c \<times>\<^sub>c \<nat>\<^sub>c) (\<nat>\<^sub>c\<^bsup>\<nat>\<^sub>c\<^esup>)) \<circ>\<^sub>c \<langle>\<langle>lower, upper\<rangle>, f\<rangle> = \<t>"
+    using assms(3) left_cart_proj_cfunc_prod leq_infix_def by (etcs_assocr, typecheck_cfuncs, auto)
+  
+  have "((indexed_sum \<circ>\<^sub>c \<langle>\<langle>left_cart_proj \<nat>\<^sub>c \<nat>\<^sub>c \<circ>\<^sub>c  left_cart_proj (\<nat>\<^sub>c \<times>\<^sub>c \<nat>\<^sub>c) (\<nat>\<^sub>c\<^bsup>\<nat>\<^sub>c\<^esup>),
+          right_cart_proj (\<nat>\<^sub>c \<times>\<^sub>c \<nat>\<^sub>c) (\<nat>\<^sub>c\<^bsup>\<nat>\<^sub>c\<^esup>)\<rangle>,monus2 \<circ>\<^sub>c swap \<nat>\<^sub>c \<nat>\<^sub>c \<circ>\<^sub>c left_cart_proj (\<nat>\<^sub>c \<times>\<^sub>c \<nat>\<^sub>c) (\<nat>\<^sub>c\<^bsup>\<nat>\<^sub>c\<^esup>)\<rangle>) \<amalg>
+     (zero \<circ>\<^sub>c \<beta>\<^bsub>(\<nat>\<^sub>c \<times>\<^sub>c \<nat>\<^sub>c) \<times>\<^sub>c \<nat>\<^sub>c\<^bsup>\<nat>\<^sub>c\<^esup>\<^esub>) \<circ>\<^sub>c cases (leq \<circ>\<^sub>c left_cart_proj (\<nat>\<^sub>c \<times>\<^sub>c \<nat>\<^sub>c) (\<nat>\<^sub>c\<^bsup>\<nat>\<^sub>c\<^esup>))) \<circ>\<^sub>c \<langle>\<langle>lower,upper\<rangle>,f\<rangle> =  
+        ((indexed_sum \<circ>\<^sub>c \<langle>\<langle>left_cart_proj \<nat>\<^sub>c \<nat>\<^sub>c \<circ>\<^sub>c  left_cart_proj (\<nat>\<^sub>c \<times>\<^sub>c \<nat>\<^sub>c) (\<nat>\<^sub>c\<^bsup>\<nat>\<^sub>c\<^esup>),
+      right_cart_proj (\<nat>\<^sub>c \<times>\<^sub>c \<nat>\<^sub>c) (\<nat>\<^sub>c\<^bsup>\<nat>\<^sub>c\<^esup>)\<rangle>, monus2 \<circ>\<^sub>c swap \<nat>\<^sub>c \<nat>\<^sub>c\<circ>\<^sub>c left_cart_proj (\<nat>\<^sub>c \<times>\<^sub>c \<nat>\<^sub>c) (\<nat>\<^sub>c\<^bsup>\<nat>\<^sub>c\<^esup>)\<rangle>) \<amalg>
+     (zero \<circ>\<^sub>c \<beta>\<^bsub>(\<nat>\<^sub>c \<times>\<^sub>c \<nat>\<^sub>c) \<times>\<^sub>c \<nat>\<^sub>c\<^bsup>\<nat>\<^sub>c\<^esup>\<^esub>)) \<circ>\<^sub>c
+     cases (leq \<circ>\<^sub>c left_cart_proj (\<nat>\<^sub>c \<times>\<^sub>c \<nat>\<^sub>c) (\<nat>\<^sub>c\<^bsup>\<nat>\<^sub>c\<^esup>)) \<circ>\<^sub>c \<langle>\<langle>lower,upper\<rangle>,f\<rangle>"
+    by(etcs_assocr, typecheck_cfuncs)
+  also have "... = ((indexed_sum \<circ>\<^sub>c \<langle>\<langle>left_cart_proj \<nat>\<^sub>c \<nat>\<^sub>c \<circ>\<^sub>c  left_cart_proj (\<nat>\<^sub>c \<times>\<^sub>c \<nat>\<^sub>c) (\<nat>\<^sub>c\<^bsup>\<nat>\<^sub>c\<^esup>),
+      right_cart_proj (\<nat>\<^sub>c \<times>\<^sub>c \<nat>\<^sub>c) (\<nat>\<^sub>c\<^bsup>\<nat>\<^sub>c\<^esup>)\<rangle>,monus2 \<circ>\<^sub>c swap \<nat>\<^sub>c \<nat>\<^sub>c \<circ>\<^sub>c left_cart_proj (\<nat>\<^sub>c \<times>\<^sub>c \<nat>\<^sub>c) (\<nat>\<^sub>c\<^bsup>\<nat>\<^sub>c\<^esup>)\<rangle>) \<amalg>
+     (zero \<circ>\<^sub>c \<beta>\<^bsub>(\<nat>\<^sub>c \<times>\<^sub>c \<nat>\<^sub>c) \<times>\<^sub>c \<nat>\<^sub>c\<^bsup>\<nat>\<^sub>c\<^esup>\<^esub>) \<circ>\<^sub>c
+     (left_coproj ((\<nat>\<^sub>c \<times>\<^sub>c \<nat>\<^sub>c) \<times>\<^sub>c \<nat>\<^sub>c\<^bsup>\<nat>\<^sub>c\<^esup>) ((\<nat>\<^sub>c \<times>\<^sub>c \<nat>\<^sub>c) \<times>\<^sub>c \<nat>\<^sub>c\<^bsup>\<nat>\<^sub>c\<^esup>))) \<circ>\<^sub>c \<langle>\<langle>lower,upper\<rangle>,f\<rangle>"
+    by (etcs_assocr,typecheck_cfuncs, simp add: True_case true_case)
+  also have "... = indexed_sum \<circ>\<^sub>c \<langle>\<langle>left_cart_proj \<nat>\<^sub>c \<nat>\<^sub>c \<circ>\<^sub>c  left_cart_proj (\<nat>\<^sub>c \<times>\<^sub>c \<nat>\<^sub>c) (\<nat>\<^sub>c\<^bsup>\<nat>\<^sub>c\<^esup>),
+      right_cart_proj (\<nat>\<^sub>c \<times>\<^sub>c \<nat>\<^sub>c) (\<nat>\<^sub>c\<^bsup>\<nat>\<^sub>c\<^esup>)\<rangle>,monus2 \<circ>\<^sub>c swap \<nat>\<^sub>c \<nat>\<^sub>c \<circ>\<^sub>c left_cart_proj (\<nat>\<^sub>c \<times>\<^sub>c \<nat>\<^sub>c) (\<nat>\<^sub>c\<^bsup>\<nat>\<^sub>c\<^esup>)\<rangle> \<circ>\<^sub>c \<langle>\<langle>lower,upper\<rangle>,f\<rangle>"
+    by (etcs_assocl, typecheck_cfuncs, metis left_coproj_cfunc_coprod)
+  also have "... = indexed_sum \<circ>\<^sub>c \<langle>\<langle>left_cart_proj \<nat>\<^sub>c \<nat>\<^sub>c \<circ>\<^sub>c  left_cart_proj (\<nat>\<^sub>c \<times>\<^sub>c \<nat>\<^sub>c) (\<nat>\<^sub>c\<^bsup>\<nat>\<^sub>c\<^esup>) \<circ>\<^sub>c \<langle>\<langle>lower,upper\<rangle>,f\<rangle>,
+      right_cart_proj (\<nat>\<^sub>c \<times>\<^sub>c \<nat>\<^sub>c) (\<nat>\<^sub>c\<^bsup>\<nat>\<^sub>c\<^esup>) \<circ>\<^sub>c \<langle>\<langle>lower,upper\<rangle>,f\<rangle>\<rangle>,monus2 \<circ>\<^sub>c swap \<nat>\<^sub>c \<nat>\<^sub>c \<circ>\<^sub>c left_cart_proj (\<nat>\<^sub>c \<times>\<^sub>c \<nat>\<^sub>c) (\<nat>\<^sub>c\<^bsup>\<nat>\<^sub>c\<^esup>) \<circ>\<^sub>c \<langle>\<langle>lower,upper\<rangle>,f\<rangle>\<rangle>"
+    using cfunc_prod_comp comp_associative2 by (typecheck_cfuncs, force)
+  also have "... =indexed_sum \<circ>\<^sub>c \<langle>\<langle>lower, f\<rangle>, monus2 \<circ>\<^sub>c swap \<nat>\<^sub>c \<nat>\<^sub>c \<circ>\<^sub>c \<langle>lower,upper\<rangle>\<rangle>"
+    using left_cart_proj_cfunc_prod right_cart_proj_cfunc_prod by (typecheck_cfuncs, auto)
+  also have "... =indexed_sum \<circ>\<^sub>c \<langle>\<langle>lower, f\<rangle>, upper \<midarrow>\<^sub>\<nat> lower\<rangle>"
+    using monus_def swap_ap by (typecheck_cfuncs, presburger)
+  then show "((indexed_sum \<circ>\<^sub>c \<langle>\<langle>left_cart_proj \<nat>\<^sub>c \<nat>\<^sub>c \<circ>\<^sub>c left_cart_proj (\<nat>\<^sub>c \<times>\<^sub>c \<nat>\<^sub>c) (\<nat>\<^sub>c\<^bsup>\<nat>\<^sub>c\<^esup>),right_cart_proj (\<nat>\<^sub>c \<times>\<^sub>c \<nat>\<^sub>c) (\<nat>\<^sub>c\<^bsup>\<nat>\<^sub>c\<^esup>)\<rangle>,monus2 \<circ>\<^sub>c swap \<nat>\<^sub>c \<nat>\<^sub>c \<circ>\<^sub>c left_cart_proj (\<nat>\<^sub>c \<times>\<^sub>c \<nat>\<^sub>c) (\<nat>\<^sub>c\<^bsup>\<nat>\<^sub>c\<^esup>)\<rangle>) \<amalg>
+     (zero \<circ>\<^sub>c \<beta>\<^bsub>(\<nat>\<^sub>c \<times>\<^sub>c \<nat>\<^sub>c) \<times>\<^sub>c \<nat>\<^sub>c\<^bsup>\<nat>\<^sub>c\<^esup>\<^esub>) \<circ>\<^sub>c cases (leq \<circ>\<^sub>c left_cart_proj (\<nat>\<^sub>c \<times>\<^sub>c \<nat>\<^sub>c) (\<nat>\<^sub>c\<^bsup>\<nat>\<^sub>c\<^esup>))) \<circ>\<^sub>c \<langle>\<langle>lower,upper\<rangle>,f\<rangle> =
+    indexed_sum \<circ>\<^sub>c \<langle>\<langle>lower,f\<rangle>,upper \<midarrow>\<^sub>\<nat> lower\<rangle>"
+    using calculation by auto
+qed
+
+
+lemma sum_uppr_eq_lwr:
+  assumes "lower \<in>\<^sub>c \<nat>\<^sub>c"  
+  assumes "f \<in>\<^sub>c \<nat>\<^sub>c\<^bsup>\<nat>\<^sub>c\<^esup>"
+  shows "summation \<circ>\<^sub>c \<langle>\<langle>lower, lower\<rangle>, f\<rangle> = cnufatem f \<circ>\<^sub>c lower"
+  shows "indexed_sum \<circ>\<^sub>c \<langle>\<langle>n, f\<rangle>, zero\<rangle> =  cnufatem f \<circ>\<^sub>c n"
+
+
+
+
+
+
+
+
+
+
+
 
 
 
